FreydSSA/Utils.lean
@@ -1,0 +1,19 @@
+import Mathlib.Data.List.MinMax
+
+theorem List.argmax_map [Preorder β] [DecidableRel λ l r: β => l < r] (Γ: List α) (f: α → β)
+  : (Γ.argmax f).map f = (Γ.map f).maximum := by
+  simp only [map_cons, maximum, argmax, foldl]
+  generalize hbase: @none α = base
+  have hbase': @none β = base.map f := by simp [<-hbase]
+  rw [hbase']
+  clear hbase hbase'
+  induction Γ generalizing base with
+  | nil => rfl
+  | cons a Γ I =>
+    rw [List.map_cons, List.foldl_cons, List.foldl_cons, I]
+    congr
+    cases base with
+    | some base =>
+      simp only [argAux, id_eq, Option.map_some']
+      split <;> rfl
+    | none => rfl
